theories/LambdaWt/WtTactic.v
@@ -14,6 +14,7 @@ Section simple_dep_types.
 
   Variable Esymbol : type Tsymbol -> Type.
   Variable EsymbolD : forall t, Esymbol t -> typeD TsymbolD t.
+  Variable Esymbol_eq_dec : forall t (a b : Esymbol t), {a = b} + {a <> b}.
 
   Section logicT.
     Variable tyProp : type Tsymbol.
@@ -73,7 +74,6 @@ Section simple_dep_types.
 
     (** NOTE: [logicT] does not form a monad due to the generalization
      **       over the indices.
-
      **)
     Definition logicT : Type :=
       forall tus tvs
@@ -86,10 +86,12 @@ Section simple_dep_types.
           * Inst Esymbol tus'
           * migrator Esymbol tus tus' }%type.
 
-    Variable PreD : forall {tus tvs}, Pre tus tvs ->
-                                      exprT TsymbolD tus tvs (typeD TsymbolD tyProp).
-    Variable PostD : forall {tus tvs}, Post tus tvs ->
-                                       exprT TsymbolD tus tvs (typeD TsymbolD tyProp).
+    Variable PreD
+    : forall {tus tvs}, Pre tus tvs ->
+                        exprT TsymbolD tus tvs (typeD TsymbolD tyProp).
+    Variable PostD
+    : forall {tus tvs}, Post tus tvs ->
+                        exprT TsymbolD tus tvs (typeD TsymbolD tyProp).
     Variable mD : forall T (TD : T -> Prop), m T -> Prop.
 
     Variable tyProp_to_Prop : typeD TsymbolD tyProp -> Prop.
@@ -112,6 +114,171 @@ Section simple_dep_types.
                                              (@PreD  _ _ goal us  vs))))))
            result.
   End logicT.
+
+  Require Import MirrorCore.LambdaWt.Unify.
+
+  Section assumption_tactic.
+    Variable tyProp : type Tsymbol.
+    Variable m : Type -> Type.
+    Require Import ExtLib.Structures.Monads.
+    Require Import ExtLib.Structures.Functor.
+    Context {Monad_m : Monad m}.
+    Context {MonadPlus_m : MonadPlus m}.
+    Context {MonadZero_m : MonadZero m}.
+    Context {Functor_m : Functor m}.
+
+    Variable unify : Unifier Esymbol (Inst Esymbol).
+    Variable unifyOk : UnifierOk (@Inst_lookup _ Esymbol) unify.
+
+    Variable mD : forall T (TD : T -> Prop), m T -> Prop.
+    Variable forall_prop : forall (T : Type),
+        (T -> typeD TsymbolD tyProp) ->
+        typeD TsymbolD tyProp.
+    Variable impl_prop :
+        typeD TsymbolD tyProp ->
+        typeD TsymbolD tyProp ->
+        typeD TsymbolD tyProp.
+
+    Variable tyProp_to_Prop : typeD TsymbolD tyProp -> Prop.
+    Variable Prop_to_tyProp : Prop -> typeD TsymbolD tyProp.
+
+    Hypothesis mD_mzero : forall T (P : T -> _), mD P mzero.
+    Hypothesis mD_fmap : forall T U (f : T -> U) (P Q : _ -> Prop) x,
+        (forall x, Q x -> P (f x)) ->
+        mD Q x ->
+        mD P (fmap f x).
+    Hypothesis mD_mplus : forall T U (P : T -> Prop) (Q : U -> Prop)
+                                 (x : m T) (y : m U),
+        mD P x ->
+        mD Q y ->
+        mD (fun x => match x with
+                     | inl x => P x
+                     | inr x => Q x
+                     end) (mplus x y).
+    Hypothesis mD_bind : forall T U (P : T -> Prop) (Q : U -> Prop) c k,
+        mD P c ->
+        (forall x, P x -> mD Q (k x)) ->
+        mD Q (bind c k).
+    Hypothesis mD_ret : forall T (P : T -> Prop) x,
+        P x -> mD P (ret x).
+
+    Hypothesis mD_conseq : forall T (P Q : T -> Prop) x,
+        mD Q x ->
+        (forall x, Q x -> P x) ->
+        mD P x.
+
+    Theorem mD_mjoin : forall T (P : T -> Prop) x y,
+        mD P x ->
+        mD P y ->
+        mD P (mjoin x y).
+    Proof.
+      unfold mjoin.
+      intros. eapply mD_bind. eapply mD_mplus.
+      eassumption. eassumption.
+      simpl. destruct x0; eauto using mD_ret.
+    Qed.
+
+    Section find_premise.
+      Context {tus : list (Tuvar Tsymbol)}.
+      Context {tvs : list (type Tsymbol)}.
+      Variables (gl : wtexpr Esymbol tus tvs tyProp)
+                (s : Inst Esymbol tus).
+
+      Fixpoint find_premise
+               (prems : list (wtexpr Esymbol tus tvs tyProp))
+      : m (Inst Esymbol tus) :=
+        match prems with
+        | nil => mzero
+        | p :: ps =>
+          match @unify _ _ _ gl p s
+          with
+          | None => find_premise ps
+          | Some s' => mjoin (ret s') (find_premise ps)
+          end
+        end.
+
+      Local Lemma find_premise_sound
+      : forall prems,
+          mD (fun inst' : Inst Esymbol tus =>
+                let trans := migrator_id Esymbol tus in
+                SubstWt.Inst_evolves trans inst' s /\
+                foralls_uvar_prop
+                  (fun
+                      us : hlist
+                             (fun tst : list (type Tsymbol) * type Tsymbol =>
+                                hlist (typeD TsymbolD) (fst tst) -> typeD TsymbolD (snd tst))
+                             tus =>
+                      InstD EsymbolD inst' us ->
+                      tyProp_to_Prop
+                        (foralls_prop tyProp forall_prop
+                                      (fun vs : hlist (typeD TsymbolD) tvs =>
+                                         impls_prop tyProp impl_prop
+                                                    (map
+                                                       (fun p : wtexpr Esymbol tus tvs tyProp =>
+                                                          wtexprD EsymbolD p us vs) prems)
+                                                    (wtexprD EsymbolD gl us vs)))))
+             (find_premise prems).
+      Proof.
+        induction prems.
+        { eapply mD_mzero. }
+        { simpl.
+          lazymatch goal with
+          | |- mD ?X _ =>
+            assert (mD X (find_premise prems))
+          end.
+          { clear - IHprems. admit. }
+          clear IHprems.
+          destruct (unify gl a s) eqn:?; eauto.
+          eapply mD_mjoin; eauto.
+          { eapply mD_ret. simpl.
+            admit. } }
+      Admitted.
+
+    End find_premise.
+
+    Definition Assumption
+    : logicT tyProp m
+             (fun tus tvs => wtexpr Esymbol tus tvs tyProp)
+             (fun _ _ => unit) :=
+      fun tus tvs prems sub goal =>
+        fmap (F:=m)
+             (fun sub' => @existT _ _ tus (tt,prems,sub',migrator_id _ _))
+             (find_premise goal sub prems).
+
+    Theorem Assumption_sound
+    : logicT_spec forall_prop impl_prop
+                  (fun tus tvs e => wtexprD EsymbolD e)
+                  (fun _ _ _ => Pure_exprT (Prop_to_tyProp True))
+                  mD tyProp_to_Prop Assumption.
+    Proof.
+      red. unfold Assumption. intros.
+      subst.
+      eapply mD_fmap
+      with (Q:=fun inst' =>
+                 let trans := migrator_id _ _ in
+                 SubstWt.Inst_evolves trans inst' inst /\
+                 foralls_uvar_prop
+                   (fun
+                       us : hlist
+                              (fun tst : list (type Tsymbol) * type Tsymbol =>
+                                 hlist (typeD TsymbolD) (fst tst) ->
+                                 typeD TsymbolD (snd tst)) tus =>
+                       InstD EsymbolD inst' us ->
+                       tyProp_to_Prop
+                         (foralls_prop tyProp forall_prop
+                                       (fun vs : hlist (typeD TsymbolD) tvs =>
+                                          impls_prop tyProp impl_prop
+                                                     (map
+                                                        (fun p : wtexpr Esymbol tus tvs tyProp =>
+                                                           wtexprD EsymbolD p us vs) prems)
+                                                     (wtexprD EsymbolD goal us vs))))).
+      { destruct 1.
+        split; [ assumption | ].
+        admit. }
+      eapply find_premise_sound.
+    Admitted.
+  End assumption_tactic.
+
 End simple_dep_types.
 
 
